DeBruijnSSA/BinSyntax/Rewrite/Term/Compose/Completeness.lean
@@ -1,0 +1,54 @@
+import DeBruijnSSA.BinSyntax.Rewrite.Term.Compose.Seq
+import DeBruijnSSA.BinSyntax.Rewrite.Term.Compose.Sum
+import DeBruijnSSA.BinSyntax.Typing.Region.Structural
+
+
+namespace BinSyntax
+
+variable [Φ: EffInstSet φ (Ty α) ε] [PartialOrder α] [SemilatticeSup ε] [OrderBot ε]
+
+namespace Term
+
+def Eqv.pack_sum {Γ : Ctx α ε} (R : LCtx α) (i : Fin R.length) : Eqv φ ((R.get i, ⊥)::Γ) (R.pack, ⊥)
+  := match R with
+  | [] => i.elim0
+  | _::R => i.cases (inl nil) (λi => inr (pack_sum R i))
+
+theorem Eqv.pack_sum_def {Γ : Ctx α ε} {R : LCtx α} {i : Fin R.length}
+  : Eqv.pack_sum (φ := φ) (Γ := Γ) R i = ⟦Term.InS.pack0 R i⟧ := by
+  induction R generalizing Γ with
+  | nil => exact i.elim0
+  | cons _ _ I =>
+    cases i using Fin.cases with
+    | zero => rfl
+    | succ i =>
+      simp only [pack_sum, I, inr_quot, Fin.cases_succ]
+      apply congrArg
+      ext
+      simp [Term.pack0, Term.Wf.pack0, -Function.iterate_succ, Function.iterate_succ']
+
+def Eqv.pack {Γ : Ctx α ε} : Eqv φ Γ (Γ.pack, Γ.sup_effect) := match Γ with
+  | [] => unit ⊥
+  | V::Γ => pair (var 0 (by cases V; simp)) ((pack (Γ := Γ)).wk0.wk_eff (by simp))
+
+def _root_.BinSyntax.Ctx.Pure.packE {Γ : Ctx α ε} (h : Γ.Pure) : Eqv φ Γ (Γ.pack, ⊥) := match Γ with
+  | [] => Eqv.unit ⊥
+  | V::Γ => Eqv.pair (Eqv.var 0 (by cases V; convert h.head; simp)) h.tail.packE.wk0
+
+def Eqv.unpack {Γ Δ : Ctx α ε} (i : Fin Γ.length) : Eqv φ ((Γ.pack, ⊥)::Δ) ((Γ.get i).1, e)
+  := match Γ with
+  | [] => i.elim0
+  | V::Γ => let2
+    (var (V := (V.1.prod (Ctx.pack Γ), e)) 0 (by simp [Ctx.pack]))
+    (i.cases (var 1 (by simp)) (λi => unpack i))
+
+-- TODO: wk lift unpack
+
+-- TODO: let1 pack (unpack i) = var i
+
+-- TODO: need InS version for this... :(
+
+-- def Subst.Eqv.unpacked {Γ Δ : Ctx α ε} (i : Fin Γ.length) : Subst.Eqv φ ((Γ.pack, ⊥)::Δ) Γ
+--   := sorry
+
+end Term
